Working towards a tiny xor example.

CircuitBuild.dfy
@@ -1,6 +1,91 @@
 module CircuitBuild {
 
+    import opened Std.Wrappers
     import opened Circuit
     import opened CircuitPath
+    import CS = CircuitStuff
+
+    // Proove that there are no loops in a small circuit.
+    // Take a set of HPNP.
+    // Step backwards to get a new set.
+    // So that after X steps the new set is empty.
+
+    function StepBack(c: Circuit, n: HPNP): (r: set<HPNP>)
+        requires CircuitValid(c)
+        requires CircuitComplete(c)
+        requires HPNPValid(c, n)
+        ensures forall m :: m in r ==> HPNPValid(c, m)
+    {
+        if HPNPValidInput(c, n) then
+            {INPtoONP(c, n)}
+        else
+            ONPtoINP(c, n)
+    }
+
+    lemma StepBackMatchesHPNPConnected(c: Circuit, n: HPNP)
+        requires CircuitValid(c)
+        requires CircuitComplete(c)
+        requires HPNPValid(c, n)
+        ensures forall m :: m in StepBack(c, n) <==> HPNPConnected(c, n, m)
+    {
+        reveal HPNPConnected();
+        reveal HPNPItoOConnected();
+        reveal HPNPOtoIConnected();
+        reveal INPtoONP();
+        forall m: HPNP
+            ensures m in StepBack(c, n) <==> HPNPConnected(c, n, m)
+        {
+            HPNPNotBothValidInputOutput(c, n);
+            if HPNPValid(c, m) {
+                HPNPNotBothValidInputOutput(c, m);
+                if HPNPValidInput(c, n) && HPNPValidOutput(c, m) {
+                    var o := INPtoONP(c, n);
+                    assert m in StepBack(c, n) <==> HPNPConnected(c, n, m);
+                }
+            }
+        }
+    }
+
+    ghost function StepSetBackInternal(c: Circuit, in_ns: set<HPNP>, out_ns: set<HPNP>): (r: set<HPNP>)
+        requires CircuitValid(c)
+        requires CircuitComplete(c)
+        requires forall n :: n in in_ns ==> HPNPValid(c, n)
+        requires forall n :: n in out_ns ==> HPNPValid(c, n)
+        ensures forall n :: n in r ==> HPNPValid(c, n)
+    {
+        if |in_ns| == 0 then
+            out_ns
+        else
+            var n :| n in in_ns;
+            var connected := StepBack(c, n);
+            assert forall m :: m in connected ==> HPNPValid(c, m);
+            var new_in_ns := in_ns - {n};
+            var new_out_ns := out_ns + connected;
+            StepSetBackInternal(c, new_in_ns, new_out_ns)
+    }
+
+    lemma StepBackEquiv(c: Circuit, n: HPNP)
+        requires CircuitValid(c)
+        requires CircuitComplete(c)
+        requires HPNPValid(c, n)
+        ensures
+            var g := CtoG(c);
+            DG.DigraphValid(g) &&
+            DG.NodeValid(g, n) &&
+            (StepBack(c, n) == DG.StepBack(g, n))
+    {
+        var g := CtoG(c);
+        CtoGValid(c);
+        reveal CtoG();
+        assert DG.DigraphValid(g);
+        HPNPInBound(c, n);
+        assert DG.NodeValid(g, n);
+        reveal HPNPConnected();
+        reveal HPNPItoOConnected();
+        reveal HPNPOtoIConnected();
+        StepBackMatchesHPNPConnected(c, n);
+        assert forall m :: m in DG.StepBack(g, n) ==> g.IsConnected(n, m);
+        assert forall m :: m in StepBack(c, n) ==> g.IsConnected(n, m);
+    }
 
 }
