CircuitStuff.dfy
@@ -6,90 +6,35 @@ module CircuitStuff {
     import opened CircuitPath
     import DG
 
-    function {:opaque} INPtoONP(c: Circuit, inp: HPNP): (onp: HPNP)
-        requires CircuitValid(c)
-        requires CircuitComplete(lib, c)
-        requires HPNPValidInput(lib, c, inp)
-        ensures HPNPValidOutput(lib, c, onp)
-        ensures HPNPConnected(lib, c, inp, onp)
-    {
-        reveal HPNPConnected();
-        reveal HPNPItoOConnected();
-        reveal HPNPValidInput();
-        reveal HPNPValidOutput();
-        var inp_c := HierarchyPathCircuit(lib, c, inp.hpn.hp);
-        HPCircuitComplete(lib, c, inp.hpn.hp);
-        assert CircuitComplete(lib, inp_c);
-        var inp_inp := NP(inp.hpn.n, inp.p);
-        reveal CircuitComplete();
-        var onp_onp := inp_c.PortSource(inp_inp).value;
-        var onp := HPNP(HPNode(inp.hpn.hp, onp_onp.n), onp_onp.p);
-        reveal CircuitValid();
-        assert HPNPItoOConnected(lib, c, inp, onp);
-        onp
-    }
-
-    function {:opaque} ONPtoDeeperINP(c: Circuit, onp: HPNP): (inp: HPNP)
-        requires CircuitValid(lib, c)
-        requires HPNPValidOutput(lib, c, onp)
-        requires HPNPtoNK(lib, c, onp).CHier?
-        ensures HPNPValidInput(lib, c, inp)
-        ensures HPNPConnected(lib, c, onp, inp)
-    {
-        HPNPValidHPValid(lib, c, onp);
-        var hp_c := HierarchyPathCircuit(lib, c, onp.hpn.hp);
-        HierarchyPathCircuitValid(lib, c, onp.hpn.hp);
-        var nk := HPNPtoNK(lib, c, onp);
-        assert CNodeKindValid(lib, hp_c.HierLevel, hp_c.PortBound, nk);
-        var lower_c := HPNPtoSubcircuit(lib, c, onp);
-        reveal HPNPValidOutput();
-        // It's an output port from a hier node.
-        // It only connects to the input into the corresponding Output node in that circuit.
-        // The port number should reference an output port CNode inside the Circuit.
-        var maybe_level_nk := lower_c.NodeKind(onp.p as CNode);
-        assert maybe_level_nk.Some?;
-        assert maybe_level_nk.value.COutput?;
-        var new_hp := ExtendHierarchyPath(lib, c, onp.hpn.hp, onp.hpn.n);
-        var inp := HPNP(HPNode(new_hp, onp.p as CNode), 0);
-        reveal HPNPConnected();
-        reveal HPNPOtoIConnected();
-        assert HPNPValidOutput(lib, c, onp);
-        reveal HPNPValidInput();
-        assert HPNPValidInput(lib, c, inp);
-        assert HPNPOtoIConnected(lib, c, onp, inp);
-        assert HPNPConnected(lib, c, onp, inp);
-        inp
-    }
-
     function {:vcs_split_on_every_assert} EvaluateINP(
             c: Circuit, m: HPNP -> bool, p: DG.Path<HPNP>): bool
-        requires CircuitValid(lib, c)
-        requires CircuitComplete(lib, c)
-        requires CircuitNoLoops(lib, c)
+        requires CircuitValid(c)
+        requires CircuitComplete(c)
+        requires CircuitNoLoops(c)
         requires |p.v| > 0
-        requires HPNPValidInput(lib, c, DG.PathEnd(p))
-        requires PathValid(lib, c, p)
-        decreases NumberOfRemainingNodes(lib, c, p), 1
+        requires HPNPValidInput(c, DG.PathEnd(p))
+        requires PathValid(c, p)
+        decreases NumberOfRemainingNodes(c, p), 1
     {
         var inp := DG.PathEnd(p);
-        var onp := INPtoONP(lib, c, inp);
-        assert HPNPValidOutput(lib, c, onp);
-        var new_p := PathAppend(lib, c, p, onp);
-        NoLoopsMeansNotInPath(lib, c, p, onp);
-        NumberOfRemainingNodesDecreases(lib, c, p, onp);
-        EvaluateONP(lib, c, m, new_p)
+        var onp := INPtoONP(c, inp);
+        assert HPNPValidOutput(c, onp);
+        var new_p := PathAppend(c, p, onp);
+        NoLoopsMeansNotInPath(c, p, onp);
+        NumberOfRemainingNodesDecreases(c, p, onp);
+        EvaluateONP(c, m, new_p)
     }
 
     function {:vcs_split_on_every_assert} EvaluateONPCInput(
             c: Circuit, isigs: HPNP -> bool, p: DG.Path<HPNP>): bool
-        requires CircuitValid(lib, c)
-        requires CircuitComplete(lib, c)
-        requires CircuitNoLoops(lib, c)
+        requires CircuitValid(c)
+        requires CircuitComplete(c)
+        requires CircuitNoLoops(c)
         requires |p.v| > 0
-        requires HPNPValidOutput(lib, c, DG.PathEnd(p))
-        requires PathValid(lib, c, p)
-        requires HPNPtoNK(lib, c, DG.PathEnd(p)).CInput?
-        decreases NumberOfRemainingNodes(lib, c, p), 1
+        requires HPNPValidOutput(c, DG.PathEnd(p))
+        requires PathValid(c, p)
+        requires HPNPtoNK(c, DG.PathEnd(p)).CInput?
+        decreases NumberOfRemainingNodes(c, p), 1
     {
         var onp := DG.PathEnd(p);
         if HPLength(onp.hpn.hp) == 0 then
@@ -97,80 +42,66 @@ module CircuitStuff {
             isigs(onp)
         else
             var (hier_n, parent_hp) := HPHeadTail(onp.hpn.hp);
-            HPNPValidHPValid(lib, c, onp);
-            assert HierarchyPathValid(lib, c, parent_hp);
+            HPNPValidHPValid(c, onp);
+            assert HierarchyPathValid(c, parent_hp);
             // If it's an input inside a hier node, then it connects to
             // the input port on the hier node on the next level up.
-            var inp := HPNP(HPNode(parent_hp, hier_n), onp.hpn.n as CPort);
-            var hier_c := HierarchyPathCircuit(lib, c, parent_hp);
-            HierarchyPathCircuitValid(lib, c, parent_hp);
-            var nk := hier_c.NodeKind(inp.hpn.n).value;
-            reveal CircuitValid();
-            reveal HPNPValidInput();
-            reveal HPNPValidOutput();
-            assert CircuitNodeKindValid(lib, hier_c);
-            assert IsIPort(lib, nk, inp.p);
-            assert HPNPValidInput(lib, c, inp);
-            var g := CtoG(lib, c);
-            DG.NoLoopsMeansNoRepeats(g);
-            reveal HPNPConnected();
-            reveal HPNPOtoIConnected();
-            assert HPNPConnected(lib, c, onp, inp);
-            var new_p := PathAppend(lib, c, p, inp);
-            NumberOfRemainingNodesDecreases(lib, c , p, inp);
-            EvaluateINP(lib, c, isigs, new_p)
+            var inp := CInputONPtoINP(c, onp);
+            var new_p := PathAppend(c, p, inp);
+            NumberOfRemainingNodesDecreases(c , p, inp);
+            EvaluateINP(c, isigs, new_p)
     }
 
     function {:vcs_split_on_every_assert} EvaluateONPCHier(
             c: Circuit, isigs: HPNP -> bool, p: DG.Path<HPNP>): bool
-        requires CircuitValid(lib, c)
-        requires CircuitComplete(lib, c)
-        requires CircuitNoLoops(lib, c)
+        requires CircuitValid(c)
+        requires CircuitComplete(c)
+        requires CircuitNoLoops(c)
         requires |p.v| > 0
-        requires HPNPValidOutput(lib, c, DG.PathEnd(p))
-        requires PathValid(lib, c, p)
-        requires HPNPtoNK(lib, c, DG.PathEnd(p)).CHier?
-        decreases NumberOfRemainingNodes(lib, c, p), 1
+        requires HPNPValidOutput(c, DG.PathEnd(p))
+        requires PathValid(c, p)
+        requires HPNPtoNK(c, DG.PathEnd(p)).CHier?
+        decreases NumberOfRemainingNodes(c, p), 1
     {
         var onp := DG.PathEnd(p);
-        var inp := ONPtoDeeperINP(lib, c, onp);
-        var new_p := PathAppend(lib, c, p, inp);
-        NumberOfRemainingNodesDecreases(lib, c, p, inp);
-        EvaluateINP(lib, c, isigs, new_p)
+        var inp := CHierONPtoINP(c, onp);
+        var new_p := PathAppend(c, p, inp);
+        NumberOfRemainingNodesDecreases(c, p, inp);
+        EvaluateINP(c, isigs, new_p)
     }
 
     function EvaluateONPCComb(
             c: Circuit, isigs: HPNP -> bool, p: DG.Path<HPNP>): bool
-        requires CircuitValid(lib, c)
-        requires CircuitComplete(lib, c)
-        requires CircuitNoLoops(lib, c)
-        requires PathValid(lib, c, p)
+        requires CircuitValid(c)
+        requires CircuitComplete(c)
+        requires CircuitNoLoops(c)
+        requires PathValid(c, p)
         requires |p.v| > 0
-        requires HPNPValidOutput(lib, c, DG.PathEnd(p))
-        requires HPNPtoNK(lib, c, DG.PathEnd(p)).CComb?
-        decreases NumberOfRemainingNodes(lib, c, p), 1
+        requires HPNPValidOutput(c, DG.PathEnd(p))
+        requires HPNPtoNK(c, DG.PathEnd(p)).CComb?
+        decreases NumberOfRemainingNodes(c, p), 1
     {
         true
     }
 
     function EvaluateONP(c: Circuit, isigs: HPNP -> bool, p: DG.Path<HPNP>): bool
-        requires CircuitValid(lib, c)
-        requires CircuitComplete(lib, c)
-        requires CircuitNoLoops(lib, c)
-        requires PathValid(lib, c, p)
+        requires CircuitValid(c)
+        requires CircuitComplete(c)
+        requires CircuitNoLoops(c)
+        requires PathValid(c, p)
         requires |p.v| > 0
-        requires HPNPValidOutput(lib, c, DG.PathEnd(p))
-        decreases NumberOfRemainingNodes(lib, c, p), 2
+        requires HPNPValidOutput(c, DG.PathEnd(p))
+        decreases NumberOfRemainingNodes(c, p), 2
     {
         var onp := DG.PathEnd(p);
-        HPNPValidHPValid(lib, c, onp);
-        var hp_c := HierarchyPathCircuit(lib, c, onp.hpn.hp);
+        HPNPValidHPValid(c, onp);
+        var hp_c := HierarchyPathCircuit(c, onp.hpn.hp);
         reveal HPNPValidOutput();
         var nk := hp_c.NodeKind(onp.hpn.n).value;
         match nk
-        case CInput() => EvaluateONPCInput(lib, c, isigs, p)
-        case CHier(_) => EvaluateONPCHier(lib, c, isigs, p)
-        case CComb(_, _, _, _, _) => EvaluateONPCComb(lib, c, isigs, p)
+        case CInput() => EvaluateONPCInput(c, isigs, p)
+        case CHier(_) => EvaluateONPCHier(c, isigs, p)
+        case CComb(_, _, _, _, _) => EvaluateONPCComb(c, isigs, p)
         case CSeq() => isigs(onp)
         case CConst(v) => v
     }
