CircuitTest.dfy
@@ -3,6 +3,10 @@ module CircuitTest {
     import opened Std.Wrappers
     import C = Circuit
     import P = Primitives
+    import Std.Collections.Map
+    import CS = CircuitStuff
+    import CP = CircuitPath
+    import DG
     // Make a circuit with a single XOR gate.
 
     const circ := C.Circuit(
@@ -26,16 +30,43 @@ module CircuitTest {
     const HierLevel: nat := 0
     const PortBound: C.CPort := 4
 
-    lemma nk_xor_valid()
-        ensures C.CNodeKindValid(HierLevel, PortBound, P.nk_xor)
-    {
-        reveal C.CircuitValid();
-    }
-
     lemma CircValid()
         ensures C.CircuitValid(circ)
     {
         reveal C.CircuitValid();
+    }
+
+    lemma CircComplete()
+        ensures C.CircuitValid(circ)
+        ensures C.CircuitComplete(circ)
+    {
+        CircValid();
+        reveal C.CircuitComplete();
+    }
+
+    lemma CircNoLoops()
+        ensures C.CircuitValid(circ)
+        ensures C.CircuitComplete(circ)
+        ensures CP.CircuitNoLoops(circ)
+    {
+        CircValid();
+        CircComplete();
+    }
+
+    lemma Blah()
+    {
+        var c := circ;
+        var i0 := C.HPNP(C.HPNode(C.HP([]), 0), C.OUTPUT_PORT);
+        var i1 := C.HPNP(C.HPNode(C.HP([]), 1), C.OUTPUT_PORT);
+        var o := C.HPNP(C.HPNode(C.HP([]), 2), C.INPUT_PORT);
+        var isigs: C.HPNP -> bool := (hpnp: C.HPNP) =>
+            if hpnp == i0 then true
+            else if hpnp == i0 then true
+            else false;
+        CircValid();
+        CircComplete();
+        CircNoLoops();
+        var b := CS.EvaluateONP(c, isigs, DG.Path([]));
     }
 
 }
